Separate modules for equivalence proofs (#108)
Moving all the code that is referred to in `Implementation` to establish
the equivalence between the imperative and functional model into a
separate module `Equivalence`. The code in the new module should not be
referred to by any other module than `Implementation`.

By submitting this pull request, I confirm that my contribution is made
under the terms of the [MIT
license](https://github.com/dafny-lang/dafny/blob/master/LICENSE.txt).

src/Distributions/BernoulliExpNeg/Implementation.dfy
@@ -11,6 +11,7 @@ module BernoulliExpNeg.Implementation {
   import Interface
   import Model
   import Bernoulli
+  import Equivalence
 
   trait {:termination false} Trait extends Interface.Trait {
 
@@ -47,68 +48,21 @@ module BernoulliExpNeg.Implementation {
     {
       var k: nat := 0;
       var a := true;
-      EnsureCaseLe1LoopInvariantOnEntry(gamma, s);
+      Equivalence.EnsureCaseLe1LoopInvariantOnEntry(gamma, s);
       while a
         decreases *
-        invariant CaseLe1LoopInvariant(gamma, old(s), a, k, s)
+        invariant Equivalence.CaseLe1LoopInvariant(gamma, old(s), a, k, s)
       {
         ghost var prevK: nat := k;
         ghost var prevS := s;
         k := k + 1;
         Helper.MulMonotonic(1, gamma.denom, k, gamma.denom);
         a := BernoulliSample(Rationals.Rational(gamma.numer, k * gamma.denom));
-        EnsureCaseLe1LoopInvariantMaintained(gamma, old(s), prevK, prevS, a, k, s);
+        Equivalence.EnsureCaseLe1LoopInvariantMaintained(gamma, old(s), prevK, prevS, a, k, s);
       }
       c := k % 2 == 1;
-      EnsureCaseLe1PostCondition(gamma, old(s), k, s, c);
+      Equivalence.EnsureCaseLe1PostCondition(gamma, old(s), k, s, c);
     }
   }
 
-  opaque ghost predicate CaseLe1LoopInvariant(gamma: Rationals.Rational, oldS: Rand.Bitstream, a: bool, k: nat, s: Rand.Bitstream)
-    requires 0 <= gamma.numer <= gamma.denom
-  {
-    Model.GammaLe1Loop(gamma)((true, 0))(oldS) == Model.GammaLe1Loop(gamma)((a, k))(s)
-  }
-
-  lemma EnsureCaseLe1LoopInvariantOnEntry(gamma: Rationals.Rational, s: Rand.Bitstream)
-    requires 0 <= gamma.numer <= gamma.denom
-    ensures CaseLe1LoopInvariant(gamma, s, true, 0, s)
-  {
-    reveal CaseLe1LoopInvariant();
-  }
-
-  lemma EnsureCaseLe1LoopInvariantMaintained(gamma: Rationals.Rational, oldS: Rand.Bitstream, k: nat, s: Rand.Bitstream, a': bool, k': nat, s': Rand.Bitstream)
-    requires 0 <= gamma.numer <= gamma.denom
-    requires k' == k + 1
-    requires inv: CaseLe1LoopInvariant(gamma, oldS, true, k, s)
-    requires bernoulli: Monad.Result(a' , s') == Bernoulli.Model.Sample(gamma.numer, k' * gamma.denom)(s)
-    ensures CaseLe1LoopInvariant(gamma, oldS, a', k', s')
-  {
-    assert iter: Monad.Result((a', k'), s') == Model.GammaLe1LoopIter(gamma)((true, k))(s) by {
-      reveal bernoulli;
-    }
-    calc {
-      Model.GammaLe1Loop(gamma)((true, 0))(oldS);
-      { reveal CaseLe1LoopInvariant(); reveal inv; }
-      Model.GammaLe1Loop(gamma)((true, k))(s);
-      { reveal iter; Model.GammaLe1LoopUnroll(gamma, (true, k), s); }
-      Model.GammaLe1Loop(gamma)((a', k'))(s');
-    }
-    reveal CaseLe1LoopInvariant();
-  }
-
-  lemma EnsureCaseLe1PostCondition(gamma: Rationals.Rational, oldS: Rand.Bitstream, k: nat, s: Rand.Bitstream, c: bool)
-    requires 0 <= gamma.numer <= gamma.denom
-    requires CaseLe1LoopInvariant(gamma, oldS, false, k, s)
-    requires c <==> (k % 2 == 1)
-    ensures Monad.Result(c, s) == Model.SampleGammaLe1(gamma)(oldS)
-  {
-    calc {
-      Model.GammaLe1Loop(gamma)((true, 0))(oldS);
-      { reveal CaseLe1LoopInvariant(); }
-      Model.GammaLe1Loop(gamma)((false, k))(s);
-      { reveal Model.GammaLe1Loop(); }
-      Monad.Result((false, k), s);
-    }
-  }
 }
