src/Distributions/BernoulliExpNeg/Model.dfy
@@ -105,19 +105,5 @@ module BernoulliExpNeg.Model {
     requires 0 <= gamma.numer <= gamma.denom
     ensures Loops.WhileTerminatesAlmostSurely(GammaLe1LoopCondition, GammaLe1LoopIter(gamma))
 
-  lemma GammaLe1LoopUnroll(gamma: Rationals.Rational, ak: (bool, nat), s: Rand.Bitstream)
-    requires 0 <= gamma.numer <= gamma.denom
-    requires ak.0
-    ensures GammaLe1Loop(gamma)(ak)(s) == Monad.Bind(GammaLe1LoopIter(gamma)(ak), GammaLe1Loop(gamma))(s)
-  {
-    GammaLe1LoopTerminatesAlmostSurely(gamma);
-    calc {
-      GammaLe1Loop(gamma)(ak)(s);
-      { reveal GammaLe1Loop(); }
-      Loops.While(GammaLe1LoopCondition, GammaLe1LoopIter(gamma), ak)(s);
-      { reveal GammaLe1Loop();
-        Loops.WhileUnroll(GammaLe1LoopCondition, GammaLe1LoopIter(gamma), ak, s); }
-      Monad.Bind(GammaLe1LoopIter(gamma)(ak), GammaLe1Loop(gamma))(s);
-    }
-  }
+
 }
